src/Base.v
@@ -1,0 +1,146 @@
+From Stdlib Require Import  FSets.FMapList FSets.FSetList FSets.FMapFacts
+                            OrderedType OrderedTypeEx.
+From QuantumLib Require Import Matrix Pad Quantum.
+From Stdlib Require Import String.
+
+Declare Scope qoreo.
+
+Module Var.
+
+  Module Export V := OrderedTypeEx.UOT_to_OT (OrderedTypeEx.Nat_as_OT).
+  Definition t := V.t.
+  Definition eq_dec : forall (x y : t), {x=y} + {x <> y} := eq_nat_dec.
+  
+  Module Map := FSets.FMapList.Make(V).
+  Module MapFacts := FMapFacts.Properties(Map).
+  Module FSet := FSets.FSetList.Make(V).
+
+  #[export] Existing Instance MapFacts.F.EqualSetoid.
+
+  Definition domain {A} (m : Map.t A) : FSet.t :=
+    let f := fun x _ s => FSet.add x s in
+    Map.fold f m FSet.empty.
+
+  Definition Singleton {A} x a (m : Map.t A) : Prop :=
+    Map.Equal m (Map.add x a (Map.empty _)).
+
+End Var.
+
+Definition qref := nat.
+
+Inductive unitary :=
+| H | X | Y | Z | CNOT | SGATE | Sdag | TGATE | Tdag.
+
+
+Module Config.
+  Record t := {
+    dim : nat;
+    qstate : Matrix dim dim
+  }.
+  (* Definition add x (v : expr) (cfg : t) : t :=
+  {|
+    state := Var.Map.add x v (state cfg);
+    dim := dim cfg;
+    qstate := qstate cfg
+  |}. *)
+  (* Definition find x (cfg : t) : option expr :=
+    Var.Map.find x (state cfg). *)
+
+
+  (* Project onto the state where qubit q is in the classical state |b> *)
+  (*Definition proj q dim (b : bool) := pad_u dim q (bool_to_matrix b).*)
+  Definition measure (b : bool) (q : qref) (cfg : t) : t :=
+    let rho' := super (pad_u q (dim cfg) (bool_to_matrix b)) (qstate cfg) in
+    {|
+      dim := dim cfg;
+      qstate := rho'
+    |}.
+    
+  Definition new (b : bool) (cfg : t) : qref * t :=
+    let q := dim cfg in
+    let rho' := kron (qstate cfg) (bool_to_ket b) in
+    (q, {|
+      dim := 1 + dim cfg;
+      qstate := rho'
+    |}).
+
+  Definition apply_matrix (cfg : t) (U : Matrix (2 ^ dim cfg) (2 ^ dim cfg)) : t :=
+  {|
+    dim := dim cfg;
+    qstate := super U (qstate cfg)
+  |}.
+  
+
+  Definition epr (cfg : t) : qref * qref * t :=
+    let q1 := dim cfg in
+    let q2 := (1 + q1)%nat in
+    let bell00 := Quantum.EPRpair † × Quantum.EPRpair in
+    let rho' := kron (qstate cfg) bell00 in
+    (q1, q2, {|
+      dim := 2 + dim cfg;
+      qstate := rho'
+    |}).
+
+
+  Definition gate_to_matrix (n : nat) (U : unitary) (qs : list qref) : Matrix (2^n) (2^n) :=
+  match U, qs with
+  | H, [q] => @pad 1 q n Quantum.hadamard
+  | X, [q] => @pad 1 q n Quantum.σx
+  | Y, [q] => @pad 1 q n Quantum.σy
+  | Z, [q] => @pad 1 q n Quantum.σz
+  | CNOT, [q1; q2] => pad_ctrl n q1 q2 Quantum.σx
+  | SGATE, [q] => @pad 1 q n Quantum.Sgate
+  | Sdag, [q]  => @pad 1 q n Quantum.Sgate†
+  | TGATE, [q] => @pad 1 q n Quantum.Tgate
+  | Tdag, [q]  => @pad 1 q n Quantum.Tgate†
+  | _, _ => Zero
+  end.
+  Definition apply_gate (U : unitary) (qs : list qref) (cfg : t) : t :=
+    apply_matrix cfg (gate_to_matrix _ U qs).
+
+    
+  Lemma test1 : gate_to_matrix 2 CNOT [0;1]%nat = cnot.
+  Proof.
+    assert (H : WF_Matrix (gate_to_matrix 2 CNOT [0%nat; 1%nat])).
+    { simpl.
+      set (H0 := QuantumLib.Pad.WF_pad_ctrl 2 0 1 σx).
+      apply H0.
+      auto with wf_db.
+    }
+    prep_matrix_equality.
+    destruct x as [ | [ | [ | [ | x ]]]];
+    destruct y as [ | [ | [ | [ | y ]]]];
+      try (rewrite H; [ auto | right; simpl; lia]; fail);
+      try (rewrite H; [ auto | left; simpl; lia]; fail);
+      try lca.
+  Qed.
+
+  Lemma test2 :gate_to_matrix 1 H [0]%nat = hadamard.
+  Proof.
+    simpl. unfold pad. simpl. Msimpl; auto.
+  Qed.
+
+End Config.
+
+(* This could be instantiated in different ways. *)
+
+Module Actor.
+
+  Module Export V := OrderedTypeEx.UOT_to_OT (OrderedTypeEx.String_as_OT).
+  Definition t := V.t.
+  Definition eq_dec : forall (x y : t), {x=y} + {x <> y} := string_dec.
+  
+  Module Map := FSets.FMapList.Make(V).
+  Module MapFacts := FMapFacts.Properties(Map).
+  Module FSet := FSets.FSetList.Make(V).
+
+  #[export] Existing Instance MapFacts.F.EqualSetoid.
+
+  Definition domain {A} (m : Map.t A) : FSet.t :=
+    let f := fun x _ s => FSet.add x s in
+    Map.fold f m FSet.empty.
+
+  Definition Singleton {A} x a (m : Map.t A) : Prop :=
+    Map.Equal m (Map.add x a (Map.empty _)).
+
+End Actor.
