src/Network.v
@@ -1,0 +1,118 @@
+From Qoreo Require Import Base.
+From Qoreo Require Expr Choreography.
+
+Module Label := Choreography.Label.
+
+From Stdlib Require Lists.List.
+Import List.ListNotations.
+Open Scope list_scope.
+Require Import Stdlib.Structures.Equalities.
+
+Module Insn.
+    Inductive t :=
+    | Let : Var.t -> Expr.t -> t
+    | LetBang : Var.t -> Expr.t -> t
+    | LetPair : Var.t -> Var.t -> Expr.t -> t
+    | Send : Expr.t -> Actor.t -> t
+    | Receive : Var.t -> Actor.t ->  t
+    | EPR : Var.t -> Actor.t -> t
+    .
+
+    Definition subst (x : Var.t) (v : Expr.t) (I : t) : t :=
+        match I with
+        | Let y e => Let y (Expr.subst x v e)
+        | LetBang y e => LetBang y (Expr.subst x v e)
+        | LetPair y1 y2 e => LetPair y1 y2 (Expr.subst x v e)
+        | Send e A => Send (Expr.subst x v e) A
+        | Receive y A => Receive y A
+        | EPR y A => EPR y A
+        end.
+
+    Definition binders (I : t) : Var.FSet.t :=
+        match I with
+        | Let y _ | LetBang y _ | Receive y _ | EPR y _ => Var.FSet.singleton y
+        | LetPair y1 y2 _ => Var.FSet.add y1 (Var.FSet.singleton y2)
+        | Send _ _ => Var.FSet.empty
+        end.
+End Insn.
+
+Module Process.
+    Definition t := list Insn.t.
+
+    Fixpoint subst (x : Var.t) (v : Expr.t) (P : t) : t :=
+    match P with
+    | [] => []
+    | (I0 :: P') =>
+      let P'' := if Var.FSet.mem x (Insn.binders I0)
+                 then P'
+                 else subst x v P'
+      in
+      (Insn.subst x v I0) :: P''
+    end.
+
+
+    (* Semantics *)
+
+    Inductive step : Process.t * Config.t -> Process.t * Config.t -> Prop :=
+    | LetC : forall x e P ρ e' ρ',
+        Expr.step (e, ρ) (e', ρ') ->
+        step (Insn.Let x e :: P, ρ) (Insn.Let x e' :: P, ρ')
+    | LetB : forall x v P ρ P',
+        Expr.Val v ->
+        P' = Process.subst x v P ->
+        step (Insn.Let x v :: P, ρ) (P', ρ)
+
+    | LetBangC : forall x e P ρ e' ρ',
+        Expr.step (e, ρ) (e', ρ') ->
+        step (Insn.LetBang x e :: P, ρ) (Insn.LetBang x e' :: P, ρ')
+    | LetBangB : forall x e P ρ P',
+        P' = Process.subst x e P ->
+        step (Insn.LetBang x (Expr.Bang e) :: P, ρ) (P', ρ)
+
+    | LetPairC : forall x1 x2 e P ρ e' ρ',
+        Expr.step (e, ρ) (e', ρ') ->
+        step (Insn.LetPair x1 x2 e :: P, ρ) (Insn.LetPair x1 x2 e' :: P, ρ')
+    | LetPairP : forall x1 x2 v1 v2 P ρ P',
+        Expr.Val v1 -> Expr.Val v2 ->
+        P' = Process.subst x2 v2 (Process.subst x1 v1 P) ->
+        step (Insn.LetPair x1 x2 (Expr.Pair v1 v2) :: P, ρ) (P', ρ)
+
+    | SendC : forall e B P ρ e' ρ',
+        Expr.step (e, ρ) (e', ρ') ->
+        step (Insn.Send e B :: P, ρ) (Insn.Send e' B :: P, ρ')
+    .
+
+End Process.
+
+Module Network.
+    Definition t := Actor.Map.t (Process.t).
+
+    Inductive step : Network.t * Config.t -> Label.t -> Network.t * Config.t -> Prop :=
+
+    | Loc : forall P P' N cfg A N' cfg',
+      Actor.Map.MapsTo A P N ->
+      Process.step (P, cfg) (P', cfg') ->
+      N' = Actor.Map.add A P' N ->
+      step (N, cfg) (Label.Loc A) (N', cfg')
+
+    | Send : forall PA PB y N cfg A v B N',
+      A <> B ->
+      Actor.Map.MapsTo A (Insn.Send v B :: PA) N ->
+      Actor.Map.MapsTo B (Insn.Receive y A :: PB) N ->
+      Expr.Val v ->
+      N' = Actor.Map.add A PA (Actor.Map.add B (Process.subst y v PB) N) ->
+      
+      step (N, cfg) (Label.Send A v B) (N', cfg)
+
+    | EPR : forall x y PA PB qA qB N cfg A B N' cfg',
+      A <> B ->
+      Actor.Map.MapsTo A (Insn.EPR x B :: PA) N ->
+      Actor.Map.MapsTo B (Insn.EPR y A :: PB) N ->
+      Config.epr cfg = (qA, qB, cfg') ->
+      N' = Actor.Map.add A (Process.subst x (Expr.QRef qA) PA) (
+            Actor.Map.add B (Process.subst y (Expr.QRef qB) PB) N) ->
+
+      step (N, cfg) (Label.EPR A B) (N', cfg')
+    .
+    
+End Network.
